Strata/Languages/Core/ProgramType.lean
@@ -19,9 +19,39 @@ open Std (ToFormat Format format)
 open Lambda
 open Strata (DiagnosticModel FileRange)
 
+namespace Factory
+
+def typeCheck (C : Expression.TyContext) (T : Expression.TyEnv)
+    : Except Format Expression.TyEnv :=
+  C.functions.foldlM (fun Env func => do
+    match func.body with
+    | none => .ok Env
+    | some body =>
+      if body.freeVars.idents.all (fun k => k ∈ func.inputs.keys) then
+        -- Temporarily add formals in the context.
+        let Env := Env.pushEmptyContext
+        let Env := Env.addInNewestContext func.inputPolyTypes
+        -- Type check the body and ensure that it unifies with the return type.
+        -- let (bodyty, Env) ← infer Env body
+        let (body_typed, Env) ← LExpr.resolve C Env body
+        let bodyty := body_typed.toLMonoTy
+        let (retty, Env) ← func.outputPolyType.instantiateWithCheck C Env
+        let S ← Constraints.unify [(retty, bodyty)] Env.stateSubstInfo |>.mapError format
+        let Env := Env.updateSubst S
+        let Env := Env.popContext
+        .ok Env
+      else
+        .error f!"Function body contains free variables!\n\
+                  {func}") T
+
+end Factory
 
 namespace Program
 
+/--
+Type check the program. The function assumes that all functions registered to
+C are already well-typed.
+-/
 def typeCheck (C: Core.Expression.TyContext) (Env : Core.Expression.TyEnv) (program : Program) :
   Except DiagnosticModel (Program × Core.Expression.TyEnv) := do
     -- Push a type substitution scope to store global type variables.
